dl

DL/Basics.ec
@@ -1,4 +1,4 @@
-require import AllCore DBool Bool List Distr Aux.
+require import AllCore DBool Bool List Distr Aux Finite.
 require import CyclicGroup.
 
 import FDistr.
@@ -6,22 +6,22 @@ import FDistr.
 require import Generic_Defs_thy.
 
 
-type dl_prob = group * group.
+type dl_prob = group.
 type dl_wit  = t.
 type dl_com = group.
 type dl_resp = t.
+type dl_chal = t.
 
 
 (* Honest Vrifier  *)
-op dl_verify (p : dl_prob) (c : dl_com) (b : bool) (r : dl_resp) : bool =
- if b then p.`1 ^ r = p.`2 * c
-  else p.`1 ^ r = c.
+op dl_verify (p : dl_prob) (c : dl_com) (b : dl_chal) (r : dl_resp) : bool =
+  g ^ r = (p ^ b) * c.
 
 
-op verify_transcript = fun p (x : dl_com * bool * dl_resp) => dl_verify p x.`1 x.`2 x.`3.
+op verify_transcript = fun p (x : dl_com * dl_chal * dl_resp) => dl_verify p x.`1 x.`2 x.`3.
 
 
-op IsDL (p : dl_prob) (w : dl_wit) : bool = p.`1 ^ w = p.`2.
+op IsDL (p : dl_prob) (w : dl_wit) : bool = g ^ w = p.
 
 
 op soundness_relation    = IsDL.
@@ -34,8 +34,8 @@ clone include ZKProtocol with
   type commitment      <- dl_com,  
   type witness         <- dl_wit,
   type response        <- dl_resp,
-  type challenge       <- bool,
-  op challenge_set     <-  (false :: true :: []),
+  type challenge       <- dl_chal,
+  op challenge_set     <- (to_seq (support dt)),
   op verify_transcript <- verify_transcript,
   op soundness_relation    <- soundness_relation,
   op completeness_relation <- completeness_relation,
@@ -50,11 +50,11 @@ module HonestProver : HonestProver = {
  proc commitment(p : dl_prob, w : dl_wit) : dl_com = {  
     (pa, wa) <- (p,w);
     r <$  dt;
-    return (p.`1) ^ r;
+    return g ^ r;
  }
 
- proc response(b : bool) : dl_resp = {
-    return (if b then r + wa else r);
+ proc response(b : dl_chal) : dl_resp = {
+    return r + b * wa;
  }  
 }.
 
