DL/Completeness.ec
@@ -2,6 +2,11 @@ pragma Goals:printall.
 require import AllCore DBool Bool List Distr.
 require import Basics.
 
+require import CyclicGroup.
+
+import FDistr.
+
+
 section.
 
 
@@ -12,11 +17,8 @@ progress.
 proc. inline*.  wp. 
 rnd. wp.  rnd.  wp. 
 skip. progress.
-case (challenge00 = false). progress. smt.
-move => bf.
-have bf1 : challenge00 = true. smt.
-clear bf. rewrite bf1. simplify. 
-smt. smt.
+rewrite /verify_transcript. simplify.
+rewrite /dl_verify. simplify. smt.
 qed. 
 
 
@@ -24,7 +26,7 @@ local lemma dl_complete_ph ya wa : IsDL ya wa
    => phoare [ Completeness(HonestProver,HonestVerifier).run : arg = (ya,wa) ==> res ] = 1%r.
 move => isdl.
 proc*.
-seq 1 : (true) 1%r 1%r 1%r 0%r (r).
+seq 1 : true 1%r 1%r 1%r 0%r r.
 call (dl_complete_h ya wa). auto.
 conseq (_: true ==> true). inline*. sp.
 wp.  progress. rnd. simplify.
@@ -33,13 +35,14 @@ wp.  rnd. skip. simplify.
 progress. smt. auto. auto. auto.
 qed.
 
-
+    (* (c1 - c2) * a    *)
 lemma dl_completeness: forall (statement : dl_prob) (witness : dl_wit) &m,
-        IsDL statement witness =>
+  IsDL statement witness =>
      Pr[Completeness(HonestProver, HonestVerifier).run(statement, witness) 
             @ &m : res] = 1%r.
 progress. byphoare (_: arg = (statement, witness) ==> _);auto.
 conseq (dl_complete_ph  statement witness _). auto. 
 qed.
+
   
 end section.
